Attempt upgrade to 8.19 to fix lsp

Flow.v
@@ -75,545 +75,223 @@ Inductive result : Type :=
     | (norm r3, enorm r4) => r3 = r4
   end.
 
-Module StagesDeep.
+Inductive flow : Type :=
+  | req : precond -> flow
+  | ens : postcond -> flow
+  | seq : flow -> flow -> flow
+  (* | fexists : (Z -> flow) -> flow. *)
+  | fexists : ident -> flow -> flow.
 
-  Inductive flow : Type :=
-    | req : precond -> flow
-    | ens : postcond -> flow
-    | seq : flow -> flow -> flow
-    (* | fexists : (Z -> flow) -> flow. *)
-    | fexists : ident -> flow -> flow.
+(* Definition flow := Z -> stages. *)
 
-  (* Definition flow := Z -> stages. *)
+Infix ";;" := seq (at level 80, right associativity).
 
-  Infix ";;" := seq (at level 80, right associativity).
+Fixpoint replace_ret x f :=
+  match f with
+  | ens q => ens (fun r s h => exists old v, s x = Some v /\ ((r = v) //\\ q old) s h)
+  | req _ => f
+  | seq a b => seq a (replace_ret x b)
+  | fexists i f => fexists i (replace_ret x f)
+  end.
 
-  Fixpoint replace_ret x f :=
-    match f with
-    | ens q => ens (fun r s h => exists old v, s x = Some v /\ ((r = v) //\\ q old) s h)
-    | req _ => f
-    | seq a b => seq a (replace_ret x b)
-    | fexists i f => fexists i (replace_ret x f)
-    end.
+(* Definition replace_ret (x:ident) (f:flow) : flow := fun s1 h1 s2 h2 r =>
+  exists v, Some v = s1 x /\
+  f s1 h1 s2 h2 (norm v). *)
 
-  (* Definition replace_ret (x:ident) (f:flow) : flow := fun s1 h1 s2 h2 r =>
-    exists v, Some v = s1 x /\
-    f s1 h1 s2 h2 (norm v). *)
+(* Reserved Notation " 'sem[' t ',' s ',' h ']=>[' t1 ',' s1 ',' h1 ',' r ']' '|=' f " (at level 50, left associativity). *)
 
-  (* Reserved Notation " 'sem[' t ',' s ',' h ']=>[' t1 ',' s1 ',' h1 ',' r ']' '|=' f " (at level 50, left associativity). *)
+(* axiomatization of semantics for staged formulae *)
+Inductive satisfies : store -> heap -> store -> heap -> result -> flow -> Prop :=
 
-  (* axiomatization of semantics for staged formulae *)
-  Inductive satisfies : store -> heap -> store -> heap -> result -> flow -> Prop :=
-
-    | sem_req: forall p s1 h1 s2 h2 r,
-      s1 = s2 ->
-      (* h3 is the piece taken out satisfying p *)
-      (exists h3, h1 = hunion h2 h3 /\ hdisjoint h2 h3 /\ p s1 h3) ->
-      satisfies s1 h1 s2 h2 (norm r) (req p)
-
-    | sem_ens: forall q s1 h1 s2 h2 r h3 v,
-      s1 = s2 ->
-      (* forall v, r = norm v -> *)
-      r = norm v /\
-      (* h3 is the piece satisfying q that is addded to h1 *)
-      h2 = hunion h1 h3 /\ hdisjoint h1 h3 /\ q v s1 h3 ->
-      satisfies s1 h1 s2 h3 (norm v) (ens q)
-
-    | sem_seq: forall f1 f2 s1 h1 s2 h2 r s3 h3 r1,
-      satisfies s1 h1 s3 h3 r1 f1 ->
-      satisfies s3 h3 s2 h2 r f2 ->
-      satisfies s1 h1 s2 h2 r (seq f1 f2)
-
-    (* | sem_ex: forall s s1 h1 h2 x e r,
-      (* the reason we can't use hoas is that the binding to the existential has to appear in the stack... *)
-      (exists v, , supdate x v s, h1]=>[true, s1, h2, r] |= e) ->
-      sem[true, s, h1]=>[true, s1, h2, r] |= fun r1 => fexists x (e r1) *)
-
-    | sem_ex: forall x f s1 h1 s2 h2 r,
-      s1 x = None ->
-      satisfies s1 h1 s2 h2 r (fexists x f)
-      (* f (supdate i v s1) h1 s2 h2 r *)
-   
-    .
-
-      (* sem[true, s1, h1]=>[true, s2, h2, norm r1] |= f1 ->
-      sem[true, s2, h2]=>[c, s3, h3, r2] |= f2 ->
-      st1 = f1 r1 ->
-      st2 = f2 r1 ->
-      ff r1 = (st1;;st2) ->
-      sem[true, s1, h1]=>[c, s3, h3, r2] |= ff *)
-
-
-  (* where " 'sem[' t ',' s ',' h ']=>[' t1 ',' s1 ',' h1 ',' r ']' '|=' f " := (satisfies t s h t1 s1 h1 r f) *)
-
-  (* Module SemanticsExamples.
-
-    Definition f1 : flow := fun r => ens (fun r1 => pure (r1=1 /\ r=r1)).
-    Definition f2 : flow := fun (r:Z) => req (fun s h => s "x" = Some 1).
-
-    (* ex z; req x->z; ens[r] x->1/\r=1 *)
-    Definition f3 : flow := fun r =>
-      (* fexists "z" (req (pts "x" "z") ;; ens ((r=1) //\\ ptsval "x" 1)). *)
-      fexists "z" (req (pts "x" "z") ;; ens (fun r1 => (r=r1) //\\ ptsval "x" 1)).
-
-    Example ex_sem_f1:
-      sem[true, sempty, hempty]=>[true, sempty, hempty, norm(1)] |= f1.
-    Proof.
-      apply sem_ens with (q := fun r => pure (r=1)).
-      exists hempty.
-      heap.
-      unfold pure.
-      intuition auto.
-      unfold f1.
-      f_equal.
-      unfold pure.
-      apply functional_extensionality.
-      intros.
-      apply functional_extensionality.
-      intros.
-      apply functional_extensionality.
-      intros.
-      auto.
-      apply propositional_extensionality.
-      intuition auto.
-    Qed. *)
-
-    (* Example ex_sem_f3:
-      sem[true, (supdate "x" 2 sempty), (hupdate 2 3 hempty) ]=>[
-        true, (supdate "x" 2 sempty), (hupdate 2 1 hempty), norm(1)] |= f3.
-    Proof.
-    (* unfold f3. *)
-      apply sem_ex.
-      exists 1.
-    (* Unset Printing Notations. *)
-      apply sem_seq with (f1 := fun r => req (pts "x" "z"))
-        (f2 := fun r => ens (ptsval "x" 1))
-        (r1 := 1)
-        (h2 := hempty)
-        (s2 := (supdate "x" 2 sempty))
-      .
-      - apply sem_req.
-      exists (hupdate 2 3 hempty).
-      heap.
-      unfold pts.
-      unfold contains.
-      unfold supdate. simpl.
-      admit.
-      -
-      unfold pureconj.
-      apply sem_ens.
-      admit.
-      - auto.
-    Admitted. *)
-    (* Qed. *)
-
-  (* End SemanticsExamples. *)
-
-End StagesDeep.
-
-Module StagesShallow.
-
-  Definition flow := store -> heap -> store -> heap -> result -> Prop.
-
-  Definition req : precond -> flow := fun p s1 h1 s2 h2 r =>
-    s1 = s2 /\
+  | sem_req: forall p s1 h1 s2 h2 r,
+    s1 = s2 ->
     (* h3 is the piece taken out satisfying p *)
-    exists h3, h1 = hunion h2 h3 /\ hdisjoint h2 h3 /\ p s1 h3.
-    (* TODO only true case for now *)
+    (exists h3, h1 = hunion h2 h3 /\ hdisjoint h2 h3 /\ p s1 h3) ->
+    satisfies s1 h1 s2 h2 (norm r) (req p)
 
-  Definition ens : postcond -> flow := fun q s1 h1 s2 h2 r =>
-    s1 = s2 /\
+  | sem_ens: forall q s1 h1 s2 h2 r h3 v,
+    s1 = s2 ->
     (* forall v, r = norm v -> *)
-    exists v, r = norm v /\
+    r = norm v /\
     (* h3 is the piece satisfying q that is addded to h1 *)
-      exists h3, h2 = hunion h1 h3 /\ hdisjoint h1 h3 /\ q v s1 h3.
+    h2 = hunion h1 h3 /\ hdisjoint h1 h3 /\ q v s1 h3 ->
+    satisfies s1 h1 s2 h3 (norm v) (ens q)
 
-  Definition seq : flow -> flow -> flow := fun f1 f2 s1 h1 s2 h2 r =>
-    exists s3 h3 r1,
-    f1 s1 h1 s3 h3 r1 /\
-    f2 s3 h3 s2 h2 r.
+  | sem_seq: forall f1 f2 s1 h1 s2 h2 r s3 h3 r1,
+    satisfies s1 h1 s3 h3 r1 f1 ->
+    satisfies s3 h3 s2 h2 r f2 ->
+    satisfies s1 h1 s2 h2 r (seq f1 f2)
 
-  Infix ";;" := seq (at level 80, right associativity).
+  (* | sem_ex: forall s s1 h1 h2 x e r,
+    (* the reason we can't use hoas is that the binding to the existential has to appear in the stack... *)
+    (exists v, , supdate x v s, h1]=>[true, s1, h2, r] |= e) ->
+    sem[true, s, h1]=>[true, s1, h2, r] |= fun r1 => fexists x (e r1) *)
 
-  (* we can't use hoas for this as the existential binding has to appear in the stack *)
-  Definition fexists : ident -> flow -> flow := fun i f s1 h1 s2 h2 r =>
-    s1 i = None /\
-    exists v,
-      f (supdate i v s1) h1 s2 h2 r.
-
-  Definition replace_ret (x:ident) (f:flow) : flow := fun s1 h1 s2 h2 r =>
-    exists v, Some v = s1 x /\
-    f s1 h1 s2 h2 (norm v).
-
-  Definition empty := ens (fun r => pure True).
-
-  (* For reasoning forward from flows in the context *)
-  Ltac fstep :=
-    match goal with
-    | H : seq _ _ _ _ _ _ _ |- _ => unfold seq in H; destr H
-    | H : req _ _ _ _ _ _ |- _ => unfold req in H; destr H; subst
-    | H : ens _ _ _ _ _ _ |- _ => unfold ens in H; destr H; subst
-    | H : pureconj _ _ _ _ |- _ => unfold pureconj in H; destr H; subst
-    end.
-
-  Ltac fsteps :=
-    match goal with
-    | H : seq _ _ _ _ _ _ _ |- _ => fstep; fsteps
-    | H : req _ _ _ _ _ _ |- _ => fstep; fsteps
-    | H : ens _ _ _ _ _ _ |- _ => fstep; fsteps
-    | H : pureconj _ _ _ _ |- _ => fstep; fsteps
-    | _ => idtac
-    end.
-
-  (* Definition satisfies s1 h1 s2 h2 r (f:flow) := f s1 h1 s2 h2 r. *)
-
-  Lemma empty_noop : forall s h r,
-    empty s h s h (norm r).
-  Proof.
-    intros.
-    unfolds.
-    unfolds.
-    intuition.
-    exists r.
-    intuition.
-    exists hempty.
-    intuition heap.
-    unfolds.
-    intuition.
-  Qed.
-
-  Module SemanticsExamples.
-
-    Definition f1 : flow := ens (fun r => pure (r=1)).
-    Definition f2 : flow := req (fun s h => s "x" = Some 1).
-
-    (* ex z; req x->z; ens[r] x->1/\r=1 *)
-    Definition f3 : flow :=
-      fexists "z" (req (pts "x" "z") ;; ens (fun r => (r=1) //\\ ptsval "x" 1)).
-
-    Example ex_sem_f1:
-      f1 sempty hempty sempty hempty (norm 1).
-      (* sem[true, sempty, hempty]=>[true, sempty, hempty, norm(1)] |= f1. *)
-    Proof.
-      unfold f1.
-      unfold ens.
-      intuition auto.
-      exists 1.
-      intuition.
-      exists hempty.
-      heap.
-      unfold pure.
-      intuition auto.
-    Qed.
-
-    Example ex_sem_f3:
-      f3 (supdate "x" 2 sempty) (hupdate 2 3 hempty) 
-        (supdate "z" 3 (supdate "x" 2 sempty)) (hupdate 2 1 hempty) (norm 1).
-    Proof.
-      unfold f3.
-      unfold fexists.
-      intuition auto.
-      exists 3. (* the initial value of z in ex z. x->z, which is given *)
-      unfold seq.
-      intuition auto.
-      exists (supdate "z" 3 (supdate "x" 2 sempty)).
-      exists hempty.
-      exists (norm 5). (* ret of req, can be anything *)
-      split.
-      - unfold req.
-        intuition auto.
-        exists (hupdate 2 3 hempty).
-        heap.
-        unfold pts.
-        unfold contains.
-        rewrite supdate_other; try congruence.
-        rewrite supdate_same.
-        rewrite supdate_same.
-        eauto.
-      - unfold ens.
-        intuition auto.
-        exists 1.
-        intuition auto.
-        exists (hupdate 2 1 hempty).
-        heap.
-        unfold pureconj.
-        intuition auto.
-        unfold ptsval.
-        unfold contains.
-        rewrite supdate_other; try congruence.
-        rewrite supdate_same.
-        eauto.
-    Qed.
-
-  End SemanticsExamples.
+  | sem_ex: forall x f s1 h1 s2 h2 r,
+    s1 x = None ->
+    satisfies s1 h1 s2 h2 r (fexists x f)
+    (* f (supdate i v s1) h1 s2 h2 r *)
+  
+    (* sem[true, s1, h1]=>[true, s2, h2, norm r1] |= f1 ->
+    sem[true, s2, h2]=>[c, s3, h3, r2] |= f2 ->
+    st1 = f1 r1 ->
+    st2 = f2 r1 ->
+    ff r1 = (st1;;st2) ->
+    sem[true, s1, h1]=>[c, s3, h3, r2] |= ff *)
 
 
-(** * Hoare rules *)
-
-  (* forward rules say how to produce a staged formula from a program *)
-  Inductive forward : expr -> flow -> Prop :=
-    | fw_const: forall n,
-      forward (pconst n) (ens (fun res => (res = n) //\\ emp))
-
-    | fw_var: forall x v,
-      forward (pvar x) (ens (fun res s h => s x = Some v /\ res = v /\ emp s h))
-
-    (* | fw_deref: forall x y,
-      forward (pderef x) (fexists y (req (pts x y);;
-        ens (fun res s h => ((res = s y) //\\ pts x y) s h)))
-
-    | fw_ref: forall x y,
-      (* forward (pref x) (fexists (fun y => ens (fun r s h => contains y (s x) s h))) *)
-      forward (pref x) (fexists y (ens (fun r s h => (r = s y) /\ (pts y x s h)))) *)
-
-    | fw_let: forall x e1 e2 f1 f2 f3,
-      forward e1 f1 ->
-      forward e2 f2 ->
-      replace_ret x f1 = f3 ->
-      forward (plet x e1 e2) (fexists x (f3 ;; f2))
-
-    (* | fw_get: forall l v, 
-      forward (GET l)
-        (req (contains l v) ;;
-        (ens (fun r => (r = v) //\\ contains l v))) *)
+    (* where " 'sem[' t ',' s ',' h ']=>[' t1 ',' s1 ',' h1 ',' r ']' '|=' f " := (satisfies t s h t1 s1 h1 r f) *)
   .
 
-  Section ForwardExamples.
 
-    (* let x = 1 in x *)
-    Example ex_forward_let1:
-      exists st, forward (plet "x" (pconst 1) (pvar "x")) st.
-    Proof.
-      eexists.
-      eapply fw_let.
-      eapply fw_const.
-      eapply fw_var.
-      eauto.
-      Unshelve.
-      exact 3. (* anything is allowed it seems *)
-    Qed.
+(* Module SemanticsExamples.
 
-    (* Check ex_intro. *)
-    (* ex_intro : forall (A : Type) (P : A -> Prop) (x : A), P x -> exists y, P y *)
-    (* Print ex_forward_let1. *)
-      (* (fun st : ...) is P *)
-      (* (fexists "x" ...) is the witness x, which is what we are after *)
-      (* (fw_let "x" ...) is the existential stmt P x, which is a derivation using the rules above, whose type includes the witness *)
+  Definition f1 : flow := fun r => ens (fun r1 => pure (r1=1 /\ r=r1)).
+  Definition f2 : flow := fun (r:Z) => req (fun s h => s "x" = Some 1).
 
-  End ForwardExamples.
+  (* ex z; req x->z; ens[r] x->1/\r=1 *)
+  Definition f3 : flow := fun r =>
+    (* fexists "z" (req (pts "x" "z") ;; ens ((r=1) //\\ ptsval "x" 1)). *)
+    fexists "z" (req (pts "x" "z") ;; ens (fun r1 => (r=r1) //\\ ptsval "x" 1)).
 
-  Definition wellformed (f:flow) s1 h1 s2 h2 r :=
-    (* satisfies s1 h1 s2 h2 r f -> substore s1 s2. *)
-    f s1 h1 s2 h2 r -> substore s1 s2.
-
-  Lemma replace_ret_wellformed : forall x f s1 h1 s2 h2 v,
-    Some v = s1 x ->
-    wellformed f s1 h1 s2 h2 (norm v) ->
-    (wellformed (replace_ret x f)) s1 h1 s2 h2 (norm v).
+  Example ex_sem_f1:
+    sem[true, sempty, hempty]=>[true, sempty, hempty, norm(1)] |= f1.
   Proof.
-    intros.
-    unfold wellformed.
-    intros.
-    (* unfold satisfies in H1. *)
-    unfold replace_ret in H1; destr H1.
-    apply H0.
-    (* unfolds. *)
-    congruence.
-  Qed.
-
-  (* we could prove _wellformed lemmas for all req, ens, etc., but currently we're doing it only for the structures generated from the forward rules *)
-
-  Lemma forward_wellformed : forall e f s1 h1 s2 h2 r,
-  forward e f -> (wellformed f) s1 h1 s2 h2 r.
-  Proof.
-  intros e f s1 h1 s2 h2 r H.
-  revert s1 h1 s2 h2 r.
-  induction H; intros.
-  - unfold wellformed; intros.
-    unfold ens in H; destr H; subst.
-    apply substore_refl.
-  - unfold wellformed; intros.
-    unfold ens in H; destr H; subst.
-    apply substore_refl.
-  -
-    unfold wellformed; intros.
-    unfold fexists in H2. destruct H2 as [? [v H5]]. subst.
-    unfold seq in H5. destruct H5 as [s3 [h3 [? [Hrr Hf2]]]]. subst.
-
-    (* introduce well-formed lemma on replace_ret *)
-    pose proof (replace_ret_wellformed x f1 (supdate x v s1) h1 s3 h3 v) as Hret.
-    rewrite supdate_same in Hret.
-    assert (Some v = Some v) as triv. reflexivity.
-    specialize (Hret triv); clear triv.
-
-    (* assuming f1 is wf using the IH, replace_ret f1 is wf *)
-    specialize (IHforward1 (supdate x v s1) h1 s3 h3 (norm v)).
-    specialize (Hret IHforward1).
-    unfold wellformed in Hret.
-    specialize (Hret Hrr).
-
-    unfold wellformed in IHforward2.
-    specialize (IHforward2 s3 h3 s2 h2 r Hf2).
-
-    unfold wellformed in IHforward1.
-    unfold replace_ret in Hrr; destruct Hrr as [? [? Hf1]]; rewrite supdate_same in H1; inj H1.
-    specialize (IHforward1 Hf1).
-    assert (substore s1 (supdate x v s1)).
-    apply substore_extension; ok.
-    apply substore_trans with (s2 := supdate x v s1); ok.
-    apply substore_trans with (s2 := s3); ok.
-  Qed.
-
-  (* {ens emp} e {\phi}, 
-  SH = { (check, s1, h1, R1)   |  [check, S, h] ~~>m [check, s1, h2, R1] |= \phi }, and 
-  [S, h, e] -----> [S2, h2, R2], R2!=\bot, 
-  such that: 
-  \exists (check, s3, h3, R3) \in SH, s3 \subset s2, h3 \subset h2, R2=R1 *)
-    Theorem soundness :
-    forall se1 he1 e se2 he2 re (**) f ss1 hs1 ss2 hs2 rs,
-      bigstep se1 he1 e se2 he2 re ->
-      substore se1 ss1 ->
-      (* he1 = hs1 -> *)
-      forward e f ->
-      f ss1 hs1 ss2 hs2 rs ->
-      substore se2 ss2
-      (* /\ he2 = hs2 *)
-      /\ compatible rs re.
-    Proof.
-      intros se1 he1 e se2 he2 re
-              f ss1 hs1 ss2 hs2 rs
-              Hb.
-      revert f ss1 hs1 ss2 hs2 rs.
-      induction Hb;
-      intros f ss1 hs1 ss2 hs2 rs;
-      intros Hsub Hf Hs.
-      - (* var. the proof comes down to the fact that both spec and program read
-            s(x) and leave the heap unchanged. *)
-        inv Hf.
-        unfold ens in Hs; destr Hs. subst.
-        unfold emp in H9.
-        unfold compatible.
-        heap.
-        unfold substore in Hsub.
-        symmetry in H.
-        specialize (Hsub v x H).
-        congruence.
-      -
-        inv Hf.
-        unfold ens in Hs; destr Hs; subst.
-        unfold compatible.
-        unfold pureconj in H6.
-        intuition auto.
-
-      -
-      (* we have an IH for each subexpr *)
-      (* v is the intermediate result of evaluating e1 *)
-      (* r is the final result *)
-      (* invp Hf [H2 H4]. *)
-      inv Hf.
-      (* invp Hf [ | |Hff1 Hff2]. *)
-      (* inversion Hf as [ Hy Hz |  |Hff1 Hff2 Hz]. subst; clear Hf. *)
-      (* the spec is of the form ex x. f1[x/r];f2 *)
-      unfold fexists in Hs. destruct Hs as [Hnotin [v1 Hseq]].
-      (* see how it evaluates *)
-      unfold seq in Hseq. destruct Hseq as [s3 [h3 [? [Hrr ?]]]].
-      unfold replace_ret in Hrr; destruct Hrr as [H10 [H9 H13]].
-
-
-      (* OLD NOW FIXED now the problem is the IH requires the eval of e1 to take place in the initial stack. but due to the existential adding something to the stack, the evaluation takes place in an extended stack, so we can't apply the IH for e1 *)
-
-      (* OLD NOW FIXED the problem is the positioning of the existential has changed. in the program, it's in the e2 initial stack. in the spec, it's right at the front, in the e1 initial stack, for f1 to assign its ret value to. so somehow need to generalise it, using compiler simulation techniques? there should be an initial relation too, so the spec is allowed to execute in an extended stack. so there's a sim rel between configurations *)
-
-      (* try to meet in the middle *)
-      (* apply IHHb2. *)
-      (* with (f:=f2) (ss2:=s2) (ss1:=s2) (hs1:=hs2). *)
-      (* easy. *)
-      (* specialize (IHHb1 f1 (supdate x v s) hs1 s1 h1 (norm v) ). *)
-      pose proof (substore_extension_trans _ s ss1 v1 x Hsub Hnotin) as Hha.
-      specialize (IHHb1 f1 (supdate x v1 ss1) hs1 s3 h3 (norm H10) Hha H2 H13).
-      destruct IHHb1 as [IH1 IH2].
-      (* we know that evaluation of e1 preserves substore *)
-
-      (* now try to use IH2 *)
-      specialize (IHHb2 f2 s3 h3 ss2 hs2 rs).
-      apply IHHb2; auto.
-      apply (substore_extension_left _ s1 s3 v x IH1).
-      unfold compatible in IH2.
-      rewrite <- IH2.
-      rewrite H9.
-      rewrite supdate_same in H9.
-      rewrite supdate_same.
-      (* need to know substore (supdate x v1 ss1) H6 is preserved by all spec/f eval *)
-      (* but how to know that, as we can give any f *)
-      pose proof (forward_wellformed _ _ (supdate x v1 ss1) hs1 s3 h3 (norm H10) H2) as Hf1wf.
-      unfold wellformed in Hf1wf.
-
-      (* assert (Hpreserve : substore (supdate x v1 ss1) s3). admit. *)
-      (* apply Hf1wf. *)
-      (* unfold substore in Hpreserve. *)
-      (* apply Hpreserve. *)
-      apply Hf1wf.
-      ok.
-      rewrite supdate_same.
-      reflexivity.
-
-  (* https://xavierleroy.org/courses/EUTypes-2019/slides.pdf *)
-
-    Qed.
-
-(** * Semantic flows *)
-  Definition triple (pre:flow) (e:expr) (spec:flow) : Prop :=
-    forall s1 h1 s2 h2 r sr s0 h0 r0 s3 h3,
-        pre s0 h0 s1 h1 r0 ->
-        bigstep s1 h1 e s2 h2 r ->
-        spec s0 h0 s3 h3 sr ->
-        compatible sr r /\ h2 = h3.
-
-  Definition triple_tabula_rasa (e:expr) (spec:flow) : Prop :=
-    triple empty e spec.
-    
-    (*
-      {pre} e {spec}
-      s,h |= pre
-      s,h,e -> s1,h1,v
-      -------------------
-      s,h,e ~> s1,h1,v |= spec
-    *)
-  (* . *)
-
-  Lemma flow_det : forall s h s1 h1 r1 s2 h2 r2 (f:flow),
-      f s h s1 h1 r1 ->
-      f s h s2 h2 r2 ->
-      s1 = s2 /\ h1 = h2 /\ r1 = r2.
-  Proof.
-    intros.
-    (* destruct H. *)
-    admit.
-  Admitted.
-
-  Lemma fw_const1 : forall p n,
-    triple p (pconst n) (p ;; ens (fun res => (res = n) //\\ emp)).
-  Proof.
-    intros.
-    unfolds.
-    intros.
-    match goal with | H : bigstep _ _ _ _ _ _ |- _ => inv H end.
-    split.
-    - fstep.
-      fstep.
-      fstep.
-      unfolds.
-      ok.
-    - fstep.
-    fstep.
-    fstep.
-    specialize (flow_det s0 h0 s2 h2 r0 s3 H1 H2 p H H3).
-    destr flow_det.
-    unfolds in H4.
-    subst.
+    apply sem_ens with (q := fun r => pure (r=1)).
+    exists hempty.
     heap.
-    (* TODO substore then needs simulation relation *)
-  Abort.
+    unfold pure.
+    intuition auto.
+    unfold f1.
+    f_equal.
+    unfold pure.
+    apply functional_extensionality.
+    intros.
+    apply functional_extensionality.
+    intros.
+    apply functional_extensionality.
+    intros.
+    auto.
+    apply propositional_extensionality.
+    intuition auto.
+  Qed. *)
+
+  (* Example ex_sem_f3:
+    sem[true, (supdate "x" 2 sempty), (hupdate 2 3 hempty) ]=>[
+      true, (supdate "x" 2 sempty), (hupdate 2 1 hempty), norm(1)] |= f3.
+  Proof.
+  (* unfold f3. *)
+    apply sem_ex.
+    exists 1.
+  (* Unset Printing Notations. *)
+    apply sem_seq with (f1 := fun r => req (pts "x" "z"))
+      (f2 := fun r => ens (ptsval "x" 1))
+      (r1 := 1)
+      (h2 := hempty)
+      (s2 := (supdate "x" 2 sempty))
+    .
+    - apply sem_req.
+    exists (hupdate 2 3 hempty).
+    heap.
+    unfold pts.
+    unfold contains.
+    unfold supdate. simpl.
+    admit.
+    -
+    unfold pureconj.
+    apply sem_ens.
+    admit.
+    - auto.
+  Admitted. *)
   (* Qed. *)
 
-End StagesShallow.
+(* End SemanticsExamples. *)
+
+
+(* forward rules say how to produce a staged formula from a program *)
+Inductive forward : expr -> flow -> Prop :=
+  | fw_const: forall n,
+    forward (pconst n) (ens (fun res => (res = n) //\\ emp))
+
+  | fw_var: forall x v,
+    forward (pvar x) (ens (fun res s h => s x = Some v /\ res = v /\ emp s h))
+
+  (* | fw_deref: forall x y,
+    forward (pderef x) (fexists y (req (pts x y);;
+      ens (fun res s h => ((res = s y) //\\ pts x y) s h)))
+
+  | fw_ref: forall x y,
+    (* forward (pref x) (fexists (fun y => ens (fun r s h => contains y (s x) s h))) *)
+    forward (pref x) (fexists y (ens (fun r s h => (r = s y) /\ (pts y x s h)))) *)
+
+  | fw_let: forall x e1 e2 f1 f2 f3,
+    forward e1 f1 ->
+    forward e2 f2 ->
+    replace_ret x f1 = f3 ->
+    forward (plet x e1 e2) (fexists x (f3 ;; f2))
+
+  (* | fw_get: forall l v, 
+    forward (GET l)
+      (req (contains l v) ;;
+      (ens (fun r => (r = v) //\\ contains l v))) *)
+.
+
+(** The semantics only grows the store *)
+Definition wellformed (f:flow) s1 h1 s2 h2 r :=
+  satisfies s1 h1 s2 h2 r f -> substore s1 s2.
+  (* f s1 h1 s2 h2 r -> substore s1 s2. *)
+
+(** Replacing the return value preserves wellformedness *)
+Lemma replace_ret_wellformed : forall f x s1 h1 s2 h2 v v1,
+  Some v = s1 x ->
+  wellformed f s1 h1 s2 h2 (norm v) ->
+  wellformed (replace_ret x f) s1 h1 s2 h2 (norm v1).
+Proof.
+  intros f.
+  induction f; intros x s1 h1 s2 h2 v H Hs.
+  (* unfold wellformed. *)
+  (* intros Hs. *)
+  (* unfold satisfies in H1. *)
+  (* inv H1. *)
+  (* induction f; inv Hs; destr_all. *)
+
+(* - unfolds. intros. unfolds in Hs. apply Hs. simpl in H0. auto. *)
+
+(* 
+  
+  - unfolds. intros.
+    unfolds in Hs. apply Hs. clear Hs.
+    simpl in H0.
+    inv H0.
+    (* destr_all. *)
+    unfolds in H7.
+    (* destr_all. *)
+    subst.
+    Print sem_ens.
+    apply sem_ens with (r:=norm H4) (h2:=hunion h1 h2).
+    auto.
+    eapply H0. *)
+
+
+
+    (* heap. *)
+    (* constructor. *)
+  (* -
+  apply IHf2.
+  unfolds.
+  intros.
+  apply IHf1.
+  unfolds.
+  intros.
+  
+  unfolds in H0.
+  apply H0.
+  eapply sem_seq with (s3:=s4) (h3:=h4).
+  exact H8.
+
+  auto.
+  auto.
+  admit.
+  - admit. *)
+  Abort.
+(* Qed. *)
